Fixes in soundness proofs and semantics.

Semantics.v
@@ -17,9 +17,12 @@ Fixpoint subst (x : id) (t : term) (t' : term) {struct t'} : term :=
 Inductive value : term -> Prop := 
   | v_true : value tm_true
   | v_false : value tm_false 
-  | v_abs : forall x T t12, value (tm_abs x T t12).
+  | v_abs : forall x T t, value (tm_abs x T t).
 
-Hint Constructors value.
+Inductive untrust_value : term -> Prop :=
+  | u_value : forall v, value v -> untrust_value (tm_distrust v).
+
+Hint Constructors value untrust_value.
 
 Reserved Notation "e '==>' e'" (at level 40).
 
@@ -27,12 +30,17 @@ Inductive step : term -> term -> Prop :=
   | e_appabs : forall x T t12 v2, value v2 -> (tm_app (tm_abs x T t12) v2) ==> subst x v2 t12
   | e_app1   : forall t1 t1' t2, t1 ==> t1' -> tm_app t1 t2 ==> tm_app t1' t2
   | e_app2   : forall v1 t2 t2', value v1 -> t2 ==> t2' -> tm_app v1 t2 ==> tm_app v1 t2'
+  | e_appabsu : forall v x T t12, untrust_value v -> tm_app (tm_abs x T t12) v ==> (subst x v t12)
+  | e_app2u : forall v1 t2 t2', untrust_value v1 -> t2 ==> t2' -> tm_app v1 t2 ==> tm_app v1 t2' 
   (** other rules **)
   | e_trust1 : forall t1 t1', t1 ==> t1' -> tm_trust t1 ==> tm_trust t1'
   | e_distrust1 : forall t1 t1', t1 ==> t1' -> tm_distrust t1 ==> tm_distrust t1'
   | e_check1 : forall t1 t1', t1 ==> t1' -> tm_check t1 ==> tm_check t1'
+  | e_distrustc1 : forall v, value v -> tm_trust (tm_distrust v) ==> tm_trust v
+  | e_distrustd1 : forall v, value v -> tm_distrust (tm_distrust v) ==> tm_distrust v
+  | e_distrusta1 : forall v x T t, value v -> tm_app (tm_distrust (tm_abs x T t)) v ==> tm_distrust (tm_app (tm_abs x T t) v)
+  | e_distrusta2 : forall v x T t, untrust_value v -> tm_app (tm_distrust (tm_abs x T t)) v ==> tm_distrust (tm_app (tm_abs x T t) v)
   | e_trustv : forall t, value t -> tm_trust t ==> t
-  | e_distrustv : forall t, value t -> tm_distrust t ==> t
   | e_checkv : forall t, value t -> tm_check t ==> t
     where "t '==>' t'" := (step t t').
 
@@ -45,24 +53,33 @@ Definition step_normal_form := normal_form step.
 
 Hint Unfold normal_form step_normal_form.
 
-Remark value_dont_step : forall t, value t -> step_normal_form t.
+Remark value_dont_step : forall t, value t -> ~ exists t', t ==> t'.
 Proof.
-  intros t H Hc ; unfold step_normal_form, normal_form in *.
-  inv H ; destruct Hc ; solve by inversion.
+  intros t H Hc. inv H ; try solve by inversion 2.
+Qed.
+
+Remark untrust_value_dont_step : forall t, untrust_value t -> ~ exists t', t ==> t'.
+Proof.
+  intros t Hu Hc. inv Hu.
+  inv Hc. inv H0. apply value_dont_step in H. elim H ; eexists ; eauto.
+  inv H.
 Qed.
 
 Ltac s := f_equal ; eauto ;
   try (match goal with
          | [H : value ?X, H1 : ?X ==> _ |- _] =>
            apply value_dont_step in H
+         | [H : untrust_value ?X, H1 : ?X ==> _ |- _] =>
+           apply untrust_value_dont_step in H
          | [H : False |- _] => elim H
          | [H : ~ _ |- _] => elim H
+         | [H : tm_distrust _ ==> _ |- _] => inv H
          | [ |- ex _] => eexists ; eauto ; fail
        end) ; try solve by inversion ; unfold step_normal_form, normal_form in *.
 
 Lemma step_deterministic : forall t t', t ==> t' -> forall t'', t ==> t'' -> t' = t''.
 Proof with eauto.
-   intros t t' H ; induction H ; intros t' H2 ; inv H2 ; repeat s.
+   intros t t' H ; induction H ; intros t'' H2 ; inv H2 ; repeat s ...
 Qed.
 
 
